<?xml version="1.0" encoding="UTF-8"?>

<section xml:id="sec-logic-truth-tables" xmlns:xi="http://www.w3.org/2001/XInclude">
	<title>Truth Tables</title>

	<objectives>
		<ul>
			<li>
				<p>
					Translate between English sentences and symbolic notation.
				</p>
			</li>
			<li>
				<p>
					Use truth tables to find truth values of basic statements.
				</p>
			</li>
			<li>
				<p>
					Use truth tables to find truth values of complex statements.
				</p>
			</li>
		</ul>
	</objectives>
<subsection>
	<title>Truth Tables</title>
	<introduction>
		<p>
			In logic we can use a <term>truth table</term> to analyze a complex statement by summarizing all the possibilities and their <term>truth values</term> (true or false). To do this, we break the statement down to its smallest elements, the propositions. We can then see the outcome of the complex statement for all possible combinations of true and false for the propositions.
		</p>	
		<p>
			For example, suppose we have the following two propositions:
			<ul>
				<li>
					<p>
						<em>R</em>: You paid your rent this month.
					</p>
				</li>
				<li>
					<p>
						<em>E</em>: You paid your electric bill this month.
					</p>
				</li>
			</ul>
		</p>
		<p>
			We use these two propositions to demonstrate the truth tables for <em>not, and,</em> and <em>or.</em>
			Before reading on, make sure you have reviewed the logical symbols shown in the <xref text="title" ref="assemblage-logical-symbols"/> block of <xref ref="sec-logic-propositions"/>.
			<!--was 47% 47%-->
		</p>
			<sidebyside widths="60% 34%" margins="0% 0%" valign="middle">
				<p>
					To set up a truth table, we list all the possible truth value combinations in a systematic way. One way to do this is to make the first column half true, then half false, then cut the pattern in half with each succeeding column. For two propositions, the first two columns are shown to the right.
				</p>
				<tabular halign="center" top="minor" left="minor" right="minor" bottom="minor">
					<row header="yes">
						<cell> <m>R</m> </cell>
						<cell> <m>E</m> </cell>
						<cell> <m>R \land E </m></cell>
					</row>
					<row>
						<cell>T</cell>
						<cell>T</cell>
						<cell></cell>
					</row>
					<row>
						<cell>T</cell>
						<cell>F</cell>
						<cell></cell>
					</row>
					<row>
						<cell>F</cell>
						<cell>T</cell>
						<cell></cell>
					</row>
					<row>
						<cell>F</cell>
						<cell>F</cell>
						<cell></cell>
					</row>
				</tabular>
			</sidebyside>
	
		<p>
			The four possible combinations are
				<ul>
					<li>
						<p>
							Row 1: You have paid your rent and electric bill.
						</p>
					</li>
					<li>
						<p>
							Row 2: You have paid your rent but not your electric bill.
						</p>
					</li>
					<li>
						<p>
							Row 3: You have not paid your rent but you have paid your electric bill.
						</p>
					</li>
					<li>
						<p>
							Row 4: You haven't paid either your rent or electric bill (yet).
						</p>
					</li>
				</ul>
		</p>
		<p>
			Once we fill in the starting columns, we add additional columns for the more complex statements. We can add as many columns as needed. Below are the basic truth tables for <em>not, and,</em> and <em>or.</em>
		</p>
	</introduction>
	<subsubsection>
		<title>Truth Tables for NOT, AND, and OR</title>
		<sidebyside widths="60% 34%" margins="0% 0%" valign="middle">
			<p>
				<term>Not</term>: In the <m>\neg R</m> column, the truth value is the opposite of the value for <m>R</m>. For example, if <m>R</m> is true (you paid your rent) then <m>\neg R</m> (you did not pay your rent) is false.
			</p>
			<tabular halign="center" top="minor" left="minor" right="minor" bottom="minor">
				<row header="yes">
					<cell right="minor"><m>R</m></cell>
					<cell right="minor"><m>\neg R</m></cell>
				</row>
				<row>
					<cell right="minor">T</cell>
					<cell right="minor">F</cell>
				</row>
				<row>
					<cell right="minor">F</cell>
					<cell right="minor">T</cell>
				</row>
			</tabular>
		</sidebyside>
		<sidebyside widths="60% 34%" margins="0% 0%" valign="middle">
			<p>
				<term>And</term>: In the <m>R \land E</m> column, you must have paid both your rent and electric bill. Otherwise <m>R \land E</m> is false.
			</p>
			<tabular halign="center" top="minor" left="minor" right="minor" bottom="minor">
				<row header="yes">
					<cell right="minor"><m>R</m></cell>
					<cell right="minor"><m>E</m></cell>
					<cell right="minor"><m>R \land E</m></cell>
				</row>
				<row>
					<cell right="minor">T</cell>
					<cell right="minor">T</cell>
					<cell right="minor">T</cell>
				</row>
				<row>
					<cell right="minor">T</cell>
					<cell right="minor">F</cell>
					<cell right="minor">F</cell>
				</row>
				<row>
					<cell right="minor">F</cell>
					<cell right="minor">T</cell>
					<cell right="minor">F</cell>
				</row>
				<row>
					<cell right="minor">F</cell>
					<cell right="minor">F</cell>
					<cell right="minor">F</cell>
				</row>
			</tabular>
		</sidebyside>
		<sidebyside widths="60% 34%" margins="0% 0%" valign="middle">
			<p>
				<term>Or</term>: In the <m>R \lor E</m> column, you must have paid either your rent or electric bill, or both (inclusive or). Otherwise <m>R \lor E</m> is false.
			</p>
			<tabular halign="center" top="minor" left="minor" right="minor" bottom="minor">
					<row header="yes">
						<cell right="minor"><m>R</m></cell>
						<cell right="minor"><m>E</m></cell>
						<cell right="minor"><m>R \lor E</m></cell>
					</row>
					<row>
						<cell right="minor">T</cell>
						<cell right="minor">T</cell>
						<cell right="minor">T</cell>
					</row>
					<row>
						<cell right="minor">T</cell>
						<cell right="minor">F</cell>
						<cell right="minor">T</cell>
					</row>
					<row>
						<cell right="minor">F</cell>
						<cell right="minor">T</cell>
						<cell right="minor">T</cell>
					</row>
					<row>
						<cell right="minor">F</cell>
						<cell right="minor">F</cell>
						<cell right="minor">F</cell>
					</row>
				</tabular>
		</sidebyside>
	</subsubsection>
	<subsubsection>
		<title>Truth Tables for the Conditional</title>
		<p>
			 To understand the truth table values for a conditional statement it is really helpful to look at it in context. We used this example in <xref ref="sec-logic-propositions"/> and we'll summarize it again here. Let's say a friend tells you, <q>If you post that photo to social media, you'll lose your job.</q> Under what conditions can you say that your friend was wrong?
		</p>
		<p>
			 There are four possible outcomes:
			 <ol>
				 <li>
					 <p>
						 You post the photo and lose your job.
					 </p>
				 </li>
				 <li>
					 <p>
						 You post the photo and don't lose your job.
					 </p>
				 </li>
				 <li>
					 <p>
						 You don't post the photo and lose your job.
					 </p>
				 </li>
				 <li>
					 <p>
						 You don't post the photo and don't lose your job.
					 </p>
				 </li>
			 </ol>
		</p>
		<p>
			 The only case where you can say your friend was wrong is the second case, in which you post the photo but still keep your job.
		</p>
		<p>
			 Your friend didn't say anything about what would happen if you didn't post the photo, so you can't say the last two statements are wrong. Even if you didn't post the photo and lost your job anyway, your friend never said that you were guaranteed to keep your job if you didn't post it.
		</p>
		<p>
			The four cases above correspond to the four rows of the truth table. For this truth table we will use <m>P</m> for <q>posting the photo,</q> and <m>L</m> for <q>losing your job.</q>
		</p>
		<sidebyside widths="60% 34%" margins="0% 0%" valign="middle">
			<p>
				<term>If, then</term>: In the <m>P\rightarrow L</m> (read <q>If <m>P</m>, then <m>L</m></q>) column, the only outcome that is false is if you post the photo and don't lose your job. Otherwise <m>P\rightarrow L</m> is true.
			</p>
				<tabular halign="center" top="minor" left="minor" right="minor" bottom="minor">
				<row header="yes">
					<cell><m>P</m></cell>
					<cell><m>L</m></cell>
					<cell><m>P\rightarrow L</m></cell>
				</row>
				<row>
					<cell>T</cell>
					<cell>T</cell>
					<cell>T</cell>
				</row>
				<row>
					<cell>T</cell>
					<cell>F</cell>
					<cell>F</cell>
				</row>
				<row>
					<cell>F</cell>
					<cell>T</cell>
					<cell>T</cell>
				</row>
				<row>
					<cell>F</cell>
					<cell>F</cell>
					<cell>T</cell>
				</row>
			</tabular>
		</sidebyside>
		<p>
			If the hypothesis (the <q>if</q> part) is false, we cannot say that the statement is a lie, so the result of the third and fourth rows is true. Notice that we are using a double negation in this explanation.
		</p>
	</subsubsection>
	</subsection>
	<subsection>
		<title>Truth Tables for Complex Statements</title>
		<p>
			Truth tables really become useful when we seek to analyze complex statements composed of multiple propositions. To do so, we need truth tables with several columns. A good basic strategy in solving such problems is to work from the inside out and create a column in the table for each intermediate statement.
			Each intermediate statement (and hence column) should require only a single logical operation to compute. This can be tedious for long problems but guards against error.
		</p>
		<example>
			<!-- <statement> -->
			<p>
				Create a truth table for the statement <m>A \lor (\neg B)</m>.
			</p>
			<!-- </statement> -->
			<!-- <solution> -->
			<sidebyside widths="47% 47%" margins="0% 0%" valign="top">
				<p>
					When we create the truth table, we start with columns for the propositions, <m>A</m> and <m>B</m>. Then we add a column for <m>\neg B</m> because that is part of the final statement. Our last column is the final statement <m>A \lor (\neg B)</m>.
					It is temping to skip the column for <m>\neg B</m> and hold that intermediate value in your head as you compute <m>A \lor (\neg B)</m>. Resist this urge as skipping intermediate steps leads often leads to errors in logic later in a complex problem.
				</p>
				<tabular halign="center" top="minor" left="minor" right="minor" bottom="minor">
					<row header="yes">
						<cell><m>A</m></cell>
						<cell><m>B</m></cell>
						<cell><m>\neg B</m></cell>
						<cell><m>A \lor (\neg B)</m></cell>
					</row>
					<row>
						<cell>T</cell>
						<cell>T</cell>
						<cell></cell>
						<cell></cell>
					</row>
					<row>
						<cell>T</cell>
						<cell>F</cell>
						<cell></cell>
						<cell></cell>
					</row>
					<row>
						<cell>F</cell>
						<cell>T</cell>
						<cell></cell>
						<cell></cell>
					</row>
					<row>
						<cell>F</cell>
						<cell>F</cell>
						<cell></cell>
						<cell></cell>
					</row>
				</tabular>
		</sidebyside>
		<sidebyside widths="47% 47%" margins="0% 0%" valign="middle">
				<p>
					To complete the third column, <em>not B</em>, we take the opposite of the <em>B</em> column. Then to complete the fourth column, we only look at the <em>A</em> and the <em>not B</em> columns and compare them using <em>or</em>.
				</p>
				<tabular halign="center" top="minor" left="minor" right="minor" bottom="minor">
					<row  header="yes">
						<cell><m>A</m></cell>
						<cell><m>B</m></cell>
						<cell><m>\neg B</m></cell>
						<cell><m>A \lor (\neg B)</m></cell>
					</row>
					<row>
						<cell>T</cell>
						<cell>T</cell>
						<cell>F</cell>
						<cell>T</cell>
					</row>
					<row>
						<cell>T</cell>
						<cell>F</cell>
						<cell>T</cell>
						<cell>T</cell>
					</row>
					<row>
						<cell>F</cell>
						<cell>T</cell>
						<cell>F</cell>
						<cell>F</cell>
					</row>
					<row>
						<cell>F</cell>
						<cell>F</cell>
						<cell>T</cell>
						<cell>T</cell>
					</row>
				</tabular>
			</sidebyside>
		<!-- </solution> -->
		</example>
	</subsection>
	<subsection>
			<title>Truth Tables with Three Propositions</title>
		<p>
			To create a truth table with three propositions we need eight rows to list all possible truth combinations. First, we will determine the columns we need to get to our final statement. Next, we will fill in the first three columns using the same methodology as before. Start with half true, half false, then cut the pattern in half each time.
		</p>
		<example>
			<statement>
				<p>
					Create a truth table for the statement <m>A \land \neg(B \lor C)</m>.
				</p>
			</statement>
			<solution>
				<p>
					First, write out the columns we need. We have <m>A,\ B,\ C,</m>, then we need the statement in the parentheses, <m>(B \lor C)</m>. Then we need the negation of that column, <m> \neg(B \lor C)</m>. The last column we need is the final statement, <m>A \land \neg(B \lor C)</m>. 
				</p>
				<p>
					Here is the initial table:
				</p>
						<tabular halign= "center" top="minor" left="minor" right="minor" bottom="minor">
							<row  header="yes">
								<cell><m>A</m></cell>
								<cell><m>B</m></cell>
								<cell><m>C</m></cell>
								<cell><m>(B \lor C)</m></cell>
								<cell><m>\neg(B \lor C)</m></cell>
								<cell><m>A \land\neg(B \lor C)</m></cell>
							</row>
							<row>
								<cell>T</cell>
								<cell>T</cell>
								<cell>T</cell>
								<cell></cell>
								<cell></cell>
								<cell></cell>
							</row>
							<row>
								<cell>T</cell>
								<cell>T</cell>
								<cell>F</cell>
								<cell></cell>
								<cell></cell>
								<cell></cell>
							</row>
							<row>
								<cell>T</cell>
								<cell>F</cell>
								<cell>T</cell>
								<cell></cell>
								<cell></cell>
								<cell></cell>
							</row>
							<row>
								<cell>T</cell>
								<cell>F</cell>
								<cell>F</cell>
								<cell></cell>
								<cell></cell>
								<cell></cell>
							</row>
							<row>
								<cell>F</cell>
								<cell>T</cell>
								<cell>T</cell>
								<cell></cell>
								<cell></cell>
								<cell></cell>
							</row>
							<row>
								<cell>F</cell>
								<cell>T</cell>
								<cell>F</cell>
								<cell></cell>
								<cell></cell>
								<cell></cell>
							</row>
							<row>
								<cell>F</cell>
								<cell>F</cell>
								<cell>T</cell>
								<cell></cell>
								<cell></cell>
								<cell></cell>
							</row>
							<row>
								<cell>F</cell>
								<cell>F</cell>
								<cell>F</cell>
								<cell></cell>
								<cell></cell>
								<cell></cell>
							</row>
						</tabular>
				<p>
					Now we complete the columns one at a time. We use the <m>B</m> column and <m>C</m> column to complete <m>B \lor C</m>. Then, <m>\neg(B \lor C)</m> is the opposite of that column. For the final column we only need to look at the first and fifth columns, shaded in blue, with AND. Here is the completed table.
				</p>
						<tabular halign="center" top="minor" left="minor" right="minor" bottom="minor">
							<row  header="yes">
								<cell><m>A</m></cell>
								<cell><m>B</m></cell>
								<cell><m>C</m></cell>
								<cell><m>(B \lor C)</m></cell>
								<cell><m>\neg(B \lor C)</m></cell>
								<cell><m>A \land\neg(B \lor C)</m></cell>
							</row>
							<row>
								<cell>T</cell>
								<cell>T</cell>
								<cell>T</cell>
								<cell>T</cell>
								<cell>F</cell>
								<cell>F</cell>
							</row>
							<row>
								<cell>T</cell>
								<cell>T</cell>
								<cell>F</cell>
								<cell>T</cell>
								<cell>F</cell>
								<cell>F</cell>
							</row>
							<row>
								<cell>T</cell>
								<cell>F</cell>
								<cell>T</cell>
								<cell>T</cell>
								<cell>F</cell>
								<cell>F</cell>
							</row>
							<row>
								<cell>T</cell>
								<cell>F</cell>
								<cell>F</cell>
								<cell>F</cell>
								<cell>T</cell>
								<cell>T</cell>
							</row>
							<row>
								<cell>F</cell>
								<cell>T</cell>
								<cell>T</cell>
								<cell>T</cell>
								<cell>F</cell>
								<cell>F</cell>
							</row>
							<row>
								<cell>F</cell>
								<cell>T</cell>
								<cell>F</cell>
								<cell>T</cell>
								<cell>F</cell>
								<cell>F</cell>
							</row>
							<row>
								<cell>F</cell>
								<cell>F</cell>
								<cell>T</cell>
								<cell>T</cell>
								<cell>F</cell>
								<cell>F</cell>
							</row>
							<row>
								<cell>F</cell>
								<cell>F</cell>
								<cell>F</cell>
								<cell>F</cell>
								<cell>T</cell>
								<cell>F</cell>
							</row>
						</tabular>
				<p>
					For this statement <m>A</m> must be true and neither <m>B</m> nor <m>C</m> can be true, so <m>A \land\neg(B \lor C)</m> is only true in the fourth row. 
				</p>
			</solution>
		</example>
		<p>
			Perhaps the last example seems theoretical. What kind of application might require this kind of logic?  For an application, consider the following propositions taken from professional baseball:
		</p>
		<p>
			Let <m>A= </m> Anaheim wins, <m>B= </m> Baltimore wins, and <m>C =</m> Cleveland wins.
			Suppose that Anaheim will make the playoffs if: (1) Anaheim wins, and (2) neither Baltimore nor Cleveland wins. When will Anaheim make the playoffs?  Only in the case that the statement <m>A \land \neg(B \lor C)</m> is true!  
			As we saw above, TFF (<m>A=</m> T, <m>B=</m> F, and <m>C=</m> F) is the only scenario in which Anaheim will make the playoffs.
		</p>
		<example>
			<statement>
				<p>
					Construct a truth table for the statement <m>(m \land\neg\,p)\rightarrow r</m>.
				</p>
			</statement>
			<solution>
				<p>
					Here are the columns for the table: 
				</p>
				<tabular halign="center" top="minor" left="minor" right="minor" bottom="minor">
					<row header="yes">
						<cell><m>m</m></cell>
						<cell><m>p</m></cell>
						<cell><m>r</m></cell>
						<cell><m>\neg\,p</m></cell>
						<cell><m>m \land\neg\,p</m></cell>
						<cell><m>(m \land\neg\,p)\rightarrow r</m></cell>
					</row>
					<row>
						<cell>T</cell>
						<cell>T</cell>
						<cell>T</cell>
						<cell></cell>
						<cell></cell>
						<cell></cell>
					</row>
					<row>
						<cell>T</cell>
						<cell>T</cell>
						<cell>F</cell>
						<cell></cell>
						<cell></cell>
						<cell></cell>
					</row>
					<row>
						<cell>T</cell>
						<cell>F</cell>
						<cell>T</cell>
						<cell></cell>
						<cell></cell>
						<cell></cell>
					</row>
					<row>
						<cell>T</cell>
						<cell>F</cell>
						<cell>F</cell>
						<cell></cell>
						<cell></cell>
						<cell></cell>
					</row>
					<row>
						<cell>F</cell>
						<cell>T</cell>
						<cell>T</cell>
						<cell></cell>
						<cell></cell>
						<cell></cell>
					</row>
					<row>
						<cell>F</cell>
						<cell>T</cell>
						<cell>F</cell>
						<cell></cell>
						<cell></cell>
						<cell></cell>
					</row>
					<row>
						<cell>F</cell>
						<cell>F</cell>
						<cell>T</cell>
						<cell></cell>
						<cell></cell>
						<cell></cell>
					</row>
					<row>
						<cell>F</cell>
						<cell>F</cell>
						<cell>F</cell>
						<cell></cell>
						<cell></cell>
						<cell></cell>
					</row>
				</tabular>
				<p>
					For the fourth column, we take the opposite of <m>p</m>. Then we use the first and fourth columns to complete <m>m \land \neg/,p</m>. Next, we use columns five and three to complete our conditional statement. 
					Be careful as we must read these columns right to left to get correct conditional values. Here is the completed table:
				</p>
				<tabular halign="center" top="minor" left="minor" right="minor" bottom="minor">
					<row header="yes">
						<cell><m>m</m></cell>
						<cell><m>p</m></cell>
						<cell><m>r</m></cell>
						<cell><m>\neg\,p</m></cell>
						<cell><m>m \land\neg\,p</m></cell>
						<cell><m>(m \land\neg\,p)\rightarrow r</m></cell>
					</row>
					<row>
						<cell>T</cell>
						<cell>T</cell>
						<cell>T</cell>
						<cell>F</cell>
						<cell>F</cell>
						<cell>T</cell>
					</row>
					<row>
						<cell>T</cell>
						<cell>T</cell>
						<cell>F</cell>
						<cell>F</cell>
						<cell>F</cell>
						<cell>T</cell>
					</row>
					<row>
						<cell>T</cell>
						<cell>F</cell>
						<cell>T</cell>
						<cell>T</cell>
						<cell>T</cell>
						<cell>T</cell>
					</row>
					<row>
						<cell>T</cell>
						<cell>F</cell>
						<cell>F</cell>
						<cell>T</cell>
						<cell>T</cell>
						<cell>F</cell>
					</row>
					<row>
						<cell>F</cell>
						<cell>T</cell>
						<cell>T</cell>
						<cell>F</cell>
						<cell>F</cell>
						<cell>T</cell>
					</row>
					<row>
						<cell>F</cell>
						<cell>T</cell>
						<cell>F</cell>
						<cell>F</cell>
						<cell>F</cell>
						<cell>T</cell>
					</row>
					<row>
						<cell>F</cell>
						<cell>F</cell>
						<cell>T</cell>
						<cell>T</cell>
						<cell>F</cell>
						<cell>T</cell>
					</row>
					<row>
						<cell>F</cell>
						<cell>F</cell>
						<cell>F</cell>
						<cell>T</cell>
						<cell>F</cell>
						<cell>T</cell>
					</row>
				</tabular>
				<p>
					When <m>m</m> is true, <m>p</m> is false, and <m>r</m> is false—the fourth row of the table—then the hypothesis <m>m \land \neg\,p</m> will be true, but the conclusion (<m>r</m>) is false, resulting in an invalid conditional statement; every other case gives a true result.
				</p>
			</solution>
		</example>
		<p>
			Again, this result might seem very abstract. 
			Here is a real-life situation that could be modeled by <m>(m \land\neg\,p)\rightarrow r</m>.
		</p>
		<p>
			Suppose <m>m=</m> we order meatballs, <m>p=</m> we order pasta, and <m>r=</m> Ruba is happy.
			The statement <m>(m \land\neg\,p)\rightarrow r</m> is then, <q>if we order meatballs and don't order pasta, then Ruba is happy</q>.
			If <m>m</m> is true (we order meatballs), <m>p</m> is false (we don't order pasta), and <m>r</m> is false (Ruba is not happy), then the statement is false, because we satisfied the premise, but Ruba did not satisfy the conclusion.
			In all other cases the statement is true.
		</p>
	</subsection>

</section>